books/centaur/fgl/pathcond-aignet.lisp
@@ -31,13 +31,11 @@
 (in-package "AIGNET")
 
 (include-book "centaur/aignet/mark-impls" :dir :system)
-(include-book "centaur/misc/intstack" :dir :system)
-(include-book "centaur/aignet/semantics" :dir :system)
+(include-book "aignet-pathcond-stobj")
+(include-book "centaur/aignet/deps" :dir :System)
 (local (include-book "theory"))
 (local (std::add-default-post-define-hook :fix))
 
-(acl2::defstobj-clone pathcond-nodebits acl2::bitarr :prefix "PATHCOND-")
-(acl2::defstobj-clone pathcond-nodestack acl2::intstack :prefix "PATHCOND-")
 (acl2::defstobj-clone pathcond-memo eba :prefix "PCMEMO-")
 ;; (acl2::defstobj-clone pathcond-memo0 eba :prefix "PCMEMO0-")
 
@@ -47,56 +45,155 @@
 
 (local (in-theory (enable aignet-idp)))
 
-(fty::defalist node-bit-alist :key-type natp :val-type bitp :true-listp t)
-
-(define nbalistp (x)
-  (and (node-bit-alistp x)
-       (no-duplicatesp-equal (alist-keys x)))
-  ///
-  (defthm nbalistp-of-cons
-    (implies (and (nbalistp 
+(fty::deffixtype nbalist-stobj :pred nbalistp :fix nbalist-fix :equiv nbalist-equiv)
 
 
-(defstobj aignet-pathcond$c
-  (pathcond-nodebits$c :type bitarr)
-  (pathcond-nodestack$c :type acl2::intstack))
+(defsection nbalist-lookup
+  (local (std::set-define-current-function nbalist-lookup))
+  (local (in-theory (enable nbalist-lookup)))
 
+  (local (defthm cdr-hons-assoc-equal-when-nbalistp
+         (implies (nbalistp x)
+                  (and (iff (cdr (hons-assoc-equal n x))
+                            (hons-assoc-equal n x))
+                       (iff (bitp (cdr (hons-assoc-equal n x)))
+                            (hons-assoc-equal n x))))))
 
-(define aignet-pathcond-lookup ((id natp)
-                                pathcond-nodebits
-                                pathcond-nodestack)
-  :guard (< id (bits-length pathcond-nodebits))
-  :returns (ans acl2::maybe-bitp :rule-classes :type-prescription)
-  (and (acl2::intstack-member id pathcond-nodestack)
-       (get-bit id pathcond-nodebits)))
+  (defret maybe-bitp-of-<fn>
+    (acl2::maybe-bitp ans)
+    :hints (("goal" :cases (ans)))
+    :rule-classes :type-prescription)
 
-(define aignet-pathcond-push ((id natp)
-                              (val bitp)
-                              pathcond-nodebits
-                              pathcond-nodestack)
-  :guard (not (acl2::intstack-member id pathcond-nodestack))
-  :returns (mv new-pathcond-nodebits
-               new-pathcond-nodestack)
-  (b* ((pathcond-nodestack (acl2::intstack-push id pathond-nodestack))
-       (pathcond-nodebits (set-bit id val pathcond-nodebits)))
-    (mv pathcond-nodebits pathcond-nodestack)))
-  
+  (defret bitp-of-<fn>
+    (iff (bitp ans) ans))
+
+  (defthm nbalist-lookup-of-cons
+    (equal (nbalist-lookup id (cons (cons key val) x))
+           (b* ((rest-lookup (nbalist-lookup id x)))
+             (if (and (equal (nfix id) (nfix key))
+                      (not rest-lookup))
+                 (bfix val)
+               rest-lookup)))
+    :hints(("Goal" :in-theory (enable nbalist-fix))))
+
+  (defthm nbalist-fix-of-cons
+    (equal (nbalist-fix (cons pair x))
+           (let* ((rest (nbalist-fix x))
+                  (first-key (nfix (car pair)))
+                  (first-val (bfix (cdr pair))))
+             (if (or (not (consp pair))
+                     (nbalist-lookup first-key x))
+                 rest
+               (cons (cons first-key first-val) rest))))
+    :hints(("Goal" :in-theory (enable nbalist-fix))))
+
+  (defthmd nbalist-lookup-redef
+    (equal (nbalist-lookup k x)
+           (b* ((x (nbalist-fix x))
+                ((unless (consp x)) nil)
+                ((when (equal (nfix k) (caar x))) (cdar x)))
+             (nbalist-lookup k (cdr x))))
+    :hints(("Goal" :expand ((hons-assoc-equal (nfix k) (nbalist-fix x)))))
+    :rule-classes :definition)
+
+  (defthm nbalist-lookup-in-cdr-when-car
+    (implies (and (nbalistp x)
+                  (consp x)
+                  (equal (nfix k) (caar x)))
+             (not (nbalist-lookup k (cdr x))))
+    :hints(("Goal" :in-theory (enable nbalist-lookup nbalistp)))))
+
+(local (in-theory (disable nbalist-fix-of-acons)))
 
 (defsection aignet-pathcond-eval
   (defun-sk aignet-pathcond-eval (aignet
-                                  pathcond-nodebits
-                                  pathcond-nodestack
+                                  nbalist
                                   invals regvals)
     (forall id 
-            (implies (member id pathcond-nodestack)
-                     (equal (nth id pathcond-nodebits)
-                            (acl2::id-eval id invals regvals aignet))))
+            (implies (nbalist-lookup id nbalist)
+                     (equal (nbalist-lookup id nbalist)
+                            (id-eval id invals regvals aignet))))
     :rewrite :direct)
 
-  
+  (in-theory (disable aignet-pathcond-eval))
 
-  )
+  (defthm aignet-pathcond-eval-of-nbalist-fix
+    (equal (aignet-pathcond-eval aignet (nbalist-fix nbalist) invals regvals)
+           (aignet-pathcond-eval aignet nbalist invals regvals))
+    :hints (("goal" :cases ((aignet-pathcond-eval aignet (nbalist-fix nbalist) invals regvals)))
+            (and stable-under-simplificationp
+                 (b* ((lit (assoc 'aignet-pathcond-eval clause)))
+                   (and lit
+                        `(:expand (,lit)
+                          :use ((:instance aignet-pathcond-eval-necc
+                                 (id (aignet-pathcond-eval-witness . ,(cdr lit)))
+                                 (nbalist ,(if (eq (third lit) 'nbalist)
+                                                     '(nbalist-fix nbalist)
+                                                   'nbalist))))
+                          :in-theory (disable aignet-pathcond-eval-necc)))))))
 
+  (defthm aignet-pathcond-eval-of-cons-when-already-bound
+    (implies (nbalist-lookup key nbalist)
+             (equal (aignet-pathcond-eval aignet (cons (cons key val) nbalist)
+                                          invals regvals)
+                    (aignet-pathcond-eval aignet nbalist invals regvals)))
+    :hints (("goal" :use ((:instance aignet-pathcond-eval-of-nbalist-fix
+                           (nbalist (cons (cons key val) nbalist)))
+                          (:instance aignet-pathcond-eval-of-nbalist-fix))
+             :in-theory (disable aignet-pathcond-eval-of-nbalist-fix))))
+             
+
+  (defthm aignet-pathcond-eval-of-cons
+    (implies (and (aignet-pathcond-eval aignet nbalist invals regvals)
+                  (not (nbalist-lookup key nbalist)))
+             (iff (aignet-pathcond-eval aignet (cons (cons key val) nbalist)
+                                        invals regvals)
+                  (equal (id-eval key invals regvals aignet) (bfix val))))
+    :hints ((and stable-under-simplificationp
+                 (let ((lit (assoc 'aignet-pathcond-eval clause)))
+                   (if lit
+                       `(:expand (,lit))
+                     `(:use ((:instance aignet-pathcond-eval-necc
+                              (id key)
+                              (nbalist (cons (cons key val) nbalist))))
+                       :in-theory (disable aignet-pathcond-eval-necc)))))))
+
+  (defthm aignet-pathcond-eval-of-cons-when-already-false
+    (implies (not (aignet-pathcond-eval aignet nbalist invals regvals))
+             (not (aignet-pathcond-eval aignet (cons (cons key val) nbalist)
+                                        invals regvals)))
+    :hints (("goal" :cases ((nbalist-lookup key nbalist)))
+            (and stable-under-simplificationp
+                 (let* ((lit (assoc 'aignet-pathcond-eval clause))
+                        (witness `(aignet-pathcond-eval-witness . ,(cdr lit))))
+                   (and lit
+                        `(:expand (,lit)
+                          :cases ((equal ,witness key))
+                          :use ((:instance nbalist-lookup-of-cons
+                                 (id ,witness)
+                                 (x nbalist)))
+                          :in-theory (disable nbalist-lookup-of-cons)))))))
+
+  (defthm aignet-pathcond-eval-implies-lookup-not-opposite
+    (implies (and (aignet-pathcond-eval aignet nbalist invals regvals)
+                  (equal b (b-not (id-eval id invals regvals aignet))))
+             (not (equal (nbalist-lookup id nbalist) b)))
+    :hints (("goal" :use aignet-pathcond-eval-necc
+             :in-theory (disable aignet-pathcond-eval-necc))))
+
+  (defcong bits-equiv equal (aignet-pathcond-eval aignet nbalist invals regvals) 3
+    :hints (("Goal" :Cases ((aignet-pathcond-eval aignet nbalist invals regvals)))
+            (and stable-under-simplificationp
+                 (b* ((lit (assoc 'aignet-pathcond-eval clause))
+                      (lit-invals (fourth lit))
+                      (other-invals (if (eq lit-invals 'invals)
+                                        'acl2::invals-equiv
+                                      'invals)))
+                   `(:expand (,lit)
+                     :use ((:instance aignet-pathcond-eval-necc
+                            (id (aignet-pathcond-eval-witness . ,(cdr lit)))
+                            (invals ,other-invals)))
+                     :in-theory (disable aignet-pathcond-eval-necc)))))))
 
 
 
@@ -113,11 +210,9 @@
   ;; memo-lookup: b* binders for looking up id in memo table and returning if available
   '(define fnname ((id natp)
                    aignet
-                   pathcond-nodestack
-                   pathcond-nodebits
+                   nbalist-stobj
                    . memo-args)
      :guard (and (< id (num-fanins aignet))
-                 (< id (bits-length pathcond-nodebits))
                  . memo-guard)
      :returns returns
      :measure (nfix id)
@@ -125,10 +220,8 @@
      (b* ((id (lnfix id))
           ((when (eql id 0))
            (b* ((ans 0)) return-unmemo))
-          (boundp (acl2::intstack-member^ id pathcond-nodestack))
-          ((when boundp)
-           (b* ((ans (get-bit id pathcond-nodebits)))
-             return-unmemo))
+          (ans (nbalist-stobj-lookup id nbalist-stobj))
+          ((when ans) return-unmemo)
           (slot0 (id->slot0 id aignet))
           (type (snode->type^ slot0))
           ((unless (eql type (gate-type)))
@@ -137,7 +230,7 @@
        (b* memo-lookup
          (b* ((fanin0 (snode->fanin^ slot0))
               (bind (fnname (lit->var fanin0)
-                            aignet pathcond-nodestack pathcond-nodebits . memo-args))
+                            aignet nbalist-stobj . memo-args))
               (f0-res ans)
               (slot1 (id->slot1 id aignet))
               (and-gate-p (eql (snode->regp^ slot1) 0))
@@ -151,7 +244,7 @@
                  return-memo))
               (fanin1 (snode->fanin^ slot1))
               (bind (fnname (lit->var fanin1)
-                            aignet pathcond-nodestack pathcond-nodebits . memo-args))
+                            aignet nbalist-stobj . memo-args))
               (f1-res ans)
               ((when (and f1-res
                           (eql (b-xor f1-res (lit->neg fanin1)) 0)
@@ -221,10 +314,14 @@
              (equal (len new-pathcond-memo) (len pathcond-memo)))))
 
 
-(defsection aignet-pathcond-implies
+(local (defthm bitp-when-maybe-bitp
+         (implies (and x (acl2::maybe-bitp x))
+                  (bitp x))))
+
+(defsection aignet-pathcond-implies-logic
   (make-event
    (sublis
-    '((fnname . aignet-pathcond-implies) ;; fnname: obvious
+    '((fnname . aignet-pathcond-implies-logic) ;; fnname: obvious
       (memo-args . nil) ;; memo-args: memo tables to pass around
       (memo-guard . nil) ;; memo-guard: list of conjuncts for guard of memo-args
       (returns . (ans acl2::maybe-bitp :rule-classes :type-prescription)) ;; returns: :returns entry
@@ -234,18 +331,26 @@
       (memo-lookup . nil)) ;; memo-lookup: b* binders for looking up id in memo table and returning if available
     *aignet-pathcond-implies-template*))
   
-  (local (in-theory (enable (:i aignet-pathcond-implies))))
+  (local (std::set-define-current-function aignet-pathcond-implies-logic))
+  (local (in-theory (enable (:i aignet-pathcond-implies-logic))))
 
-  (
+  (defret eval-when-aignet-pathcond-implies-logic
+    (implies (and (aignet-pathcond-eval aignet nbalist-stobj invals regvals)
+                  ans)
+             (equal ans (id-eval id invals regvals aignet)))
+    :hints (("Goal" :induct <call>
+             :expand (<call>
+                      (aignet-pathcond-implies-logic 0 aignet nbalist-stobj)))
+            (and stable-under-simplificationp
+                 '(:expand ((id-eval id invals regvals aignet))
+                   :in-theory (enable eval-and-of-lits eval-xor-of-lits lit-eval)))))
 
-
-
-
-  )
-
-(local (defthm bitp-when-maybe-bitp
-         (implies (and x (acl2::maybe-bitp x))
-                  (bitp x))))
+  (defret aignet-pathcond-implies-logic-not-equal-negation
+    (implies (and (aignet-pathcond-eval aignet nbalist-stobj invals regvals)
+                  (equal b (b-not (id-eval id invals regvals aignet))))
+             (not (equal ans b)))
+    :hints (("goal" :use eval-when-aignet-pathcond-implies-logic
+             :in-theory (disable eval-when-aignet-pathcond-implies-logic)))))
 
 (defsection aignet-pathcond-implies-memo
   (make-event
@@ -275,35 +380,34 @@
 
 
   (defun-sk aignet-pathcond-implies-memo-cond (aignet
-                                               pathcond-nodestack
-                                               pathcond-nodebits
+                                               nbalist-stobj
                                                pathcond-memo)
     (forall id
             (b* (((mv memo-set memo-val) (aignet-pathcond-implies-memo-get
                                           id pathcond-memo)))
               (implies memo-set
                        (equal memo-val
-                              (aignet-pathcond-implies id aignet pathcond-nodestack pathcond-nodebits)))))
+                              (aignet-pathcond-implies-logic id aignet nbalist-stobj)))))
     :rewrite :direct)
 
   (local (in-theory (disable aignet-pathcond-implies-memo-cond
                              b-xor not)))
 
   (defret aignet-pathcond-implies-memo-correct
-    (implies (aignet-pathcond-implies-memo-cond aignet pathcond-nodestack pathcond-nodebits
+    (implies (aignet-pathcond-implies-memo-cond aignet nbalist-stobj
                                                 pathcond-memo)
-             (and (equal ans (aignet-pathcond-implies id aignet pathcond-nodestack pathcond-nodebits))
-                  (aignet-pathcond-implies-memo-cond aignet pathcond-nodestack pathcond-nodebits new-pathcond-memo)))
+             (and (equal ans (aignet-pathcond-implies-logic id aignet nbalist-stobj))
+                  (aignet-pathcond-implies-memo-cond aignet nbalist-stobj new-pathcond-memo)))
     :hints (("goal" :induct <call>)
             (and stable-under-simplificationp
                  (b* ((lit (assoc 'aignet-pathcond-implies-memo-cond clause))
                       (expands '(:expand (<call>
-                                          (aignet-pathcond-implies
-                                           id aignet pathcond-nodestack pathcond-nodebits)
-                                          (aignet-pathcond-implies
-                                           0 aignet pathcond-nodestack pathcond-nodebits)
+                                          (aignet-pathcond-implies-logic
+                                           id aignet nbalist-stobj)
+                                          (aignet-pathcond-implies-logic
+                                           0 aignet nbalist-stobj)
                                           (aignet-pathcond-implies-memo
-                                           0 aignet pathcond-nodestack pathcond-nodebits pathcond-memo)))))
+                                           0 aignet nbalist-stobj pathcond-memo)))))
                    (if lit
                        `(:computed-hint-replacement
                          ((and stable-under-simplificationp
@@ -315,16 +419,405 @@
 
   (defthm aignet-pathcond-implies-memo-cond-of-repeat-0
     (aignet-pathcond-implies-memo-cond aignet
-                                       pathcond-nodestack
-                                       pathcond-nodebits
+                                       nbalist-stobj
                                        (acl2::repeat n 0))
     :hints(("Goal" :in-theory (enable aignet-pathcond-implies-memo-cond
                                       aignet-pathcond-implies-memo-get)))))
 
 
 
+(local (defthm cdr-hons-assoc-under-iff-when-nbalistp
+         (implies (nbalistp x)
+                  (iff (cdr (hons-assoc-equal a x))
+                       (hons-assoc-equal a x)))))
 
-                                               
-        
+(defthm nbalistp-of-cons-when-lookup
+  (equal (nbalistp (cons a x))
+         (and (consp a)
+              (natp (car a))
+              (bitp (cdr a))
+              (not (nbalist-lookup (car a) x))
+              (nbalistp x)))
+  :hints(("Goal" :in-theory (enable nbalist-lookup))))
+
+(local (in-theory (disable nbalistp-of-cons)))
+
+(define nbalist-extension-p ((x nbalistp) (y nbalistp))
+  :measure (len (nbalist-fix x))
+  (b* ((x (nbalist-fix x)))
+    (or (equal x (nbalist-fix y))
+        (and (consp x)
+             (nbalist-extension-p (cdr x) y))))
+  ///
+  (defthm nbalist-extension-of-cons
+    (nbalist-extension-p (cons pair x) x)
+    :hints (("goal" :expand ((nbalist-extension-p (cons pair x) x)))))
+
+  (defthm nbalist-extension-transitive
+    (implies (and (nbalist-extension-p x y)
+                  (nbalist-extension-p y z))
+             (nbalist-extension-p x z)))
+
+  (defthm nbalist-lookup-in-extension
+    (implies (and (nbalist-extension-p x y)
+                  (nbalist-lookup k y))
+             (equal (nbalist-lookup k x)
+                    (nbalist-lookup k y)))
+    :hints (("goal" :induct t)
+            (and stable-under-simplificationp
+                 '(:in-theory (enable nbalist-lookup-redef)))))
+
+  (defthm nbalist-extension-implies-len-gte
+    (implies (nbalist-extension-p x y)
+             (>= (len (nbalist-fix x)) (len (nbalist-fix y))))
+    :rule-classes (:rewrite :linear))
+
+  (defthm aignet-pathcond-eval-of-extension
+    (implies (and (nbalist-extension-p x y)
+                  (not (aignet-pathcond-eval aignet y invals regvals)))
+             (not (aignet-pathcond-eval aignet x invals regvals)))
+    :hints ((and stable-under-simplificationp
+                 (let* ((lit (assoc 'aignet-pathcond-eval clause)))
+                   `(:expand (,lit)
+                     :use ((:instance aignet-pathcond-eval-necc
+                            (id (aignet-pathcond-eval-witness . ,(cdr lit)))
+                            (nbalist x)))
+                     :do-not-induct t :in-theory (disable nbalist-extension-p))))))
+
+  (defthm nbalist-extension-self
+    (nbalist-extension-p x x)))
+
+
+(define nbalist-bound ((x nbalistp))
+  :measure (len (nbalist-fix x))
+  :returns (bound natp :rule-classes :type-prescription)
+  (b* ((x (nbalist-fix x))
+       ((when (atom x)) 0))
+    (max (caar x)
+         (nbalist-bound (cdr x))))
+  ///
+  (defthmd nbalist-lookup-implies-id-lte-bound
+    (implies (nbalist-lookup id nbalist)
+             (<= (nfix id) (nbalist-bound nbalist)))
+    :hints(("Goal" :in-theory (enable nbalist-lookup-redef)))
+    :rule-classes :forward-chaining)
+
+  (defthmd nbalist-lookup-implies-id-lte-bound-natp
+    (implies (and (nbalist-lookup id nbalist)
+                  (natp id))
+             (<= id (nbalist-bound nbalist)))
+    :hints (("goal" :use nbalist-lookup-implies-id-lte-bound))
+    :rule-classes (:rewrite :forward-chaining)))
+
+(defsection nbalist-depends-on
+  (defun-sk nbalist-depends-on (v nbalist aignet)
+    (exists id
+            (and (nbalist-lookup id nbalist)
+                 (depends-on id (innum->id v aignet) aignet))))
+
+  (in-theory (disable nbalist-depends-on
+                      nbalist-depends-on-suff))
+
+  ;; (defthm nbalist-not-depends-on-implies-not-depends-on
+  ;;   (implies (and (not (nbalist-depends-on v nbalist aignet))
+  ;;                 (nbalist-lookup id aignet))
+  ;;            (not (depends-on id 
+
+  (defthm aignet-pathcond-eval-of-set-var-when-not-depends-on
+    (implies (and (not (nbalist-depends-on v nbalist aignet))
+                  (< (nfix v) (num-ins aignet)))
+             (equal (aignet-pathcond-eval aignet nbalist (update-nth v val invals) regvals)
+                    (aignet-pathcond-eval aignet nbalist invals regvals)))
+    :hints (("goal" :cases ((aignet-pathcond-eval aignet nbalist invals regvals))
+             :do-not-induct t)
+            (and stable-under-simplificationp
+                 (b* ((lit (assoc 'aignet-pathcond-eval clause)))
+                   (and lit
+                        `(:expand (,lit)
+                          :use ((:instance aignet-pathcond-eval-necc
+                                 (id (aignet-pathcond-eval-witness . ,(cdr lit)))
+                                 (invals ,(if (eq (fourth lit) 'invals)
+                                               '(update-nth v val invals)
+                                             'invals)))
+                                (:instance nbalist-depends-on-suff
+                                 (id (aignet-pathcond-eval-witness . ,(cdr lit)))))
+                          :in-theory (disable aignet-pathcond-eval-necc)))))))
+
+  (defthm nbalist-depends-on-of-cons
+    (equal (nbalist-depends-on v (cons (cons key val) nbalist) aignet)
+           (or (nbalist-depends-on v nbalist aignet)
+               (and (not (nbalist-lookup key nbalist))
+                    (depends-on key (innum->id v aignet) aignet))))
+    :hints (("goal" :cases ((nbalist-depends-on v (cons (cons key val) nbalist) aignet)))
+            (and stable-under-simplificationp
+                 (b* ((lit (assoc 'nbalist-depends-on clause))
+                      (lit-nbalist (third lit))
+                      (other-nbalist (if (eq lit-nbalist 'nbalist)
+                                         '(cons (cons key val) nbalist)
+                                       'nbalist))
+                      (other-lit (update-nth 2 other-nbalist lit)))
+                   `(:expand (,other-lit)
+                     :use ((:instance nbalist-depends-on-suff
+                            (nbalist ,lit-nbalist)
+                            (id (if (depends-on key (innum->id v aignet) aignet)
+                                    key
+                                  (nbalist-depends-on-witness . ,(cdr other-lit))))))
+                     :in-theory (disable nbalist-depends-on-suff)))))
+    :otf-flg t)
+
+  (defthm nbalist-depends-on-of-nbalist-fix
+    (equal (nbalist-depends-on v (nbalist-fix nbalist) aignet)
+           (nbalist-depends-on v nbalist aignet))
+    :hints (("goal" :cases ((nbalist-depends-on v nbalist aignet)))
+            (and stable-under-simplificationp
+                 (b* ((lit (assoc 'nbalist-depends-on clause))
+                      (lit-nbalist (third lit))
+                      (other-nbalist (if (eq lit-nbalist 'nbalist)
+                                         '(nbalist-fix nbalist)
+                                       'nbalist))
+                      (other-lit (update-nth 2 other-nbalist lit)))
+                   `(:expand (,other-lit)
+                     :use ((:instance nbalist-depends-on-suff
+                            (nbalist ,lit-nbalist)
+                            (id (nbalist-depends-on-witness . ,(cdr other-lit)))))
+                     :in-theory (disable nbalist-depends-on-suff)))))
+    :otf-flg t))
+
+
+
+;; (define nbalist-depends-on ((v natp "The input number, in this case")
+;;                             (x nbalistp)
+;;                             aignet)
+;;   :guard (and (< (nfix v) (num-ins aignet))
+;;               (< (nbalist-bound x) (num-fanins aignet)))
+;;   :guard-hints (("goal" :in-theory (enable nbalist-bound)))
+;;   :measure (len (nbalist-fix x))
+;;   (b* ((x (nbalist-fix x))
+;;        ((when (atom x)) nil))
+;;     (or (depends-on (caar x) (innum->id v aignet) aignet)
+;;         (nbalist-depends-on v (cdr x) aignet)))
+;;   ///
+
+;;   (defthm aignet-pathcond-eval-of-set-var-when-not-depends-on
+;;     (implies (not (nbalist-depends-on v nbalist aignet))
+;;              (equal (aignet-pathcond-eval nbalist aignet (update-nth v val invals) regvals)
+;;                     (aignet-pathcond-eval nbalist aignet invals regvals)))
+;;     :hints (("goal" :cases ((aignet-pathcond-eval aignet nbalist invals regvals))
+;;              :do-not-induct t)
+;;             (and stable-under-simplificationp
+;;                  (b* ((lit (assoc 'aignet-pathcond-eval clause)))
+;;                    (and lit
+;;                         `(:expand (,lit)
+;;                           :use ((:instance aignet-pathcond-eval-necc
+;;                                  (id (aignet-pathcond-eval-witness . ,(cdr lit)))
+;;                                  (nbalist ,(if (eq (fourth lit) 'invals)
+;;                                                '(update-nth v val invals)
+;;                                              'invals))))
+;;                           :in-theory (disable aignet-pathcond-eval-necc))))))))
+
+(define aignet-pathcond-assume-logic ((lit litp)
+                                aignet
+                                nbalist-stobj)
+  :guard (< (lit->var lit) (num-fanins aignet))
+  :measure (lit->var lit)
+  :returns (mv contradictionp
+               (new-nbalist-stobj nbalistp))
+  (b* ((id (lit->var lit))
+       (neg (lit->neg lit))
+       (nbalist-stobj (mbe :logic (non-exec (nbalist-fix nbalist-stobj))
+                           :exec nbalist-stobj))
+       ((when (eql 0 id))
+        (mv (eql neg 0) nbalist-stobj))
+       (look (nbalist-stobj-lookup id nbalist-stobj))
+       ((when look)
+        (mv (eql look neg) nbalist-stobj))
+       (slot0 (id->slot0 id aignet))
+       (slot1 (id->slot1 id aignet))
+       ((when (or (eql neg 1)
+                  (not (eql (snode->type slot0) (gate-type)))
+                  (eql (snode->regp slot1) 1)))
+        (b* ((nbalist-stobj (nbalist-stobj-push id (b-not neg) nbalist-stobj)))
+          (mv nil nbalist-stobj)))
+       ;; AND node -- go down the branches
+       ((mv contradictionp nbalist-stobj)
+        (aignet-pathcond-assume-logic (snode->fanin slot0) aignet nbalist-stobj))
+       ((when contradictionp) (mv contradictionp nbalist-stobj)))
+    (aignet-pathcond-assume-logic (snode->fanin slot1) aignet nbalist-stobj))
+  ///
+  (defret nbalist-assume-correct
+    (implies (and (aignet-pathcond-eval aignet nbalist-stobj invals regvals)
+                  (equal 1 (lit-eval lit invals regvals aignet)))
+             (and (not contradictionp)
+                  (aignet-pathcond-eval aignet new-nbalist-stobj invals regvals)))
+    :hints (("goal" :induct t)
+            (and stable-under-simplificationp
+                 '(:expand ((lit-eval lit invals regvals aignet))))
+            (and stable-under-simplificationp
+                 '(:expand ((id-eval (lit->var lit) invals regvals aignet))
+                   :in-theory (enable eval-and-of-lits eval-xor-of-lits)))))
+
+  (defret nbalist-assume-eval-new-calist
+    (implies (not contradictionp)
+             (equal (aignet-pathcond-eval aignet new-nbalist-stobj invals regvals)
+                    (and (aignet-pathcond-eval aignet nbalist-stobj invals regvals)
+                         (equal 1 (lit-eval lit invals regvals aignet)))))
+    :hints (("goal" :induct t)
+            (and stable-under-simplificationp
+                 '(:expand ((lit-eval lit invals regvals aignet))))
+            (and stable-under-simplificationp
+                 '(:expand ((id-eval (lit->var lit) invals regvals aignet))
+                   :in-theory (enable eval-and-of-lits eval-xor-of-lits)))))
+
+  (defret nbalist-assume-contradictionp-correct
+    (implies (and contradictionp
+                  (equal (lit-eval lit invals regvals aignet) 1))
+             (not (aignet-pathcond-eval aignet nbalist-stobj invals regvals))))
+
+  (defret nbalist-extension-of-aignet-pathcond-assume-logic
+      (nbalist-extension-p new-nbalist-stobj nbalist-stobj)
+    :hints(("Goal"
+            :induct <call>
+            :expand (<call>))))
+
+  (defret nbalist-depends-on-of-aignet-pathcond-assume-logic
+    (implies (and (not (nbalist-depends-on v nbalist-stobj aignet))
+                  (not (depends-on (lit->var lit) (innum->id v aignet) aignet)))
+             (not (nbalist-depends-on v new-nbalist-stobj aignet)))
+    :hints(("Goal"
+            :induct <call>
+            :expand (<call>)))))
+
+
+(define nbalist-stobj-rewind ((len natp)
+                              nbalist-stobj)
+  :guard (<= len (nbalist-stobj-len nbalist-stobj))
+  :measure (nbalist-stobj-len nbalist-stobj)
+  :returns (new-nbalist-stobj nbalistp)
+  (b* (((when (mbe :logic (<= (nbalist-stobj-len nbalist-stobj) (nfix len))
+                   :exec (int= (nbalist-stobj-len nbalist-stobj) len)))
+        (mbe :logic (non-exec (nbalist-fix nbalist-stobj))
+             :exec nbalist-stobj))
+       (nbalist-stobj (nbalist-stobj-pop nbalist-stobj)))
+    (nbalist-stobj-rewind len nbalist-stobj))
+  ///
+  (local (defthm nbalist-stobj-rewind-of-extension-lemma
+           (implies (nbalist-extension-p x y)
+                    (equal (nbalist-stobj-rewind (len (nbalist-fix y)) x)
+                           (nbalist-fix y)))
+           :hints(("Goal" :induct t)
+                  (and stable-under-simplificationp
+                       '(:expand ((nbalist-extension-p x y)))))))
+
+  (fty::deffixequiv nbalist-stobj-rewind)
+
+  (defthm nbalist-stobj-rewind-of-extension
+    (implies (and (nbalist-extension-p x y)
+                  (equal (nfix len) (len (nbalist-fix y))))
+             (equal (nbalist-stobj-rewind len x)
+                    (nbalist-fix y)))
+    :hints (("goal" :use ((:instance nbalist-stobj-rewind-of-extension-lemma))
+             :in-theory (disable nbalist-stobj-rewind-of-extension-lemma)
+             :do-not-induct t))))
+                  
+(defstobj aignet-pathcond$c
+  (aignet-pathcond-nbalist$c :type nbalist-stobj)
+  (aignet-pathcond-memo$c :type eba))
+
+(local (include-book "std/lists/repeat" :dir :system))
+
+(define aignet-pathcond-implies$c ((id natp)
+                                   aignet aignet-pathcond$c)
+  :enabled t
+  :guard (< id (num-fanins aignet))
+  (stobj-let
+   ((nbalist-stobj (aignet-pathcond-nbalist$c aignet-pathcond$c))
+    (pathcond-memo (aignet-pathcond-memo$c aignet-pathcond$c)))
+   (res pathcond-memo)
+   (b* ((pathcond-memo (eba-clear pathcond-memo))
+        (pathcond-memo (if (<= (eba-length pathcond-memo) (+ 1 (* 2 (lnfix id))))
+                           (resize-eba (max 16 (* 4 (lnfix id))) pathcond-memo)
+                         pathcond-memo)))
+     (aignet-pathcond-implies-memo id aignet nbalist-stobj pathcond-memo))
+   (mv res aignet-pathcond$c)))
+
+(define aignet-pathcond-implies$a ((id natp)
+                                   aignet aignet-pathcond$a)
+  :enabled t
+  :guard (< id (num-fanins aignet))
+  (mv (non-exec (aignet-pathcond-implies-logic id aignet aignet-pathcond$a))
+      aignet-pathcond$a))
+
+
+(define aignet-pathcond-assume$c ((lit litp)
+                                   aignet aignet-pathcond$c)
+  :enabled t
+  :guard (< (lit->var lit) (num-fanins aignet))
+  (stobj-let
+   ((nbalist-stobj (aignet-pathcond-nbalist$c aignet-pathcond$c))
+    (pathcond-memo (aignet-pathcond-memo$c aignet-pathcond$c)))
+   (contra nbalist-stobj pathcond-memo)
+   (b* (((mv contra nbalist-stobj)
+         (aignet-pathcond-assume-logic lit aignet nbalist-stobj))
+        (pathcond-memo (eba-clear pathcond-memo)))
+     (mv contra nbalist-stobj pathcond-memo))
+   (mv contra aignet-pathcond$c)))
+
+(define aignet-pathcond-assume$a ((lit litp)
+                                  aignet aignet-pathcond$a)
+  :enabled t
+  :guard (< (lit->var lit) (num-fanins aignet))
+  (b* (((mv contra aignet-pathcond$a) (non-exec (aignet-pathcond-assume-logic lit aignet aignet-pathcond$a))))
+    (mv contra aignet-pathcond$a)))
+
+(define aignet-pathcond-len$c (aignet-pathcond$c)
+  :enabled t
+  (stobj-let ((nbalist-stobj (aignet-pathcond-nbalist$c aignet-pathcond$c)))
+             (len)
+             (nbalist-stobj-len nbalist-stobj)
+             len))
+
+(define aignet-pathcond-len$a (aignet-pathcond$a)
+  :enabled t
+  (len (ec-call (nbalist-fix aignet-pathcond$a))))
+
+(define aignet-pathcond-rewind$c ((len natp) aignet-pathcond$c)
+  :enabled t
+  :guard (<= len (aignet-pathcond-len$c aignet-pathcond$c))
+  (stobj-let ((nbalist-stobj (aignet-pathcond-nbalist$c aignet-pathcond$c)))
+             (nbalist-stobj)
+             (nbalist-stobj-rewind len nbalist-stobj)
+             aignet-pathcond$c))
+
+(define aignet-pathcond-rewind$a ((len natp) aignet-pathcond$a)
+  :enabled t
+  :guard (<= len (aignet-pathcond-len$a aignet-pathcond$a))
+  (non-exec (nbalist-stobj-rewind len aignet-pathcond$a)))
+
+(encapsulate nil
+  (local (define aignet-pathcond-corr (aignet-pathcond$c aignet-pathcond$a)
+           :non-executable t
+           :enabled t
+           (equal aignet-pathcond$a (nth *aignet-pathcond-nbalist$c* aignet-pathcond$c))))
+
+  (local (in-theory (disable (acl2::repeat))))
+
+  (defabsstobj-events aignet-pathcond
+    :concrete aignet-pathcond$c
+    :corr-fn aignet-pathcond-corr
+    :recognizer (aignet-pathcondp :logic nbalist-stobj$ap
+                                  :exec aignet-pathcond$cp)
+    :creator (create-aignet-pathcond :logic create-nbalist-stobj$a
+                                     :exec create-aignet-pathcond$c)
+    :exports ((aignet-pathcond-implies :logic aignet-pathcond-implies$a
+                                       :exec aignet-pathcond-implies$c
+                                       :protect t)
+              (aignet-pathcond-assume :logic aignet-pathcond-assume$a
+                                           :exec aignet-pathcond-assume$c
+                                           :protect t)
+              (aignet-pathcond-len :logic aignet-pathcond-len$a
+                                   :exec aignet-pathcond-len$c)
+              (aignet-pathcond-rewind :logic aignet-pathcond-rewind$a
+                                      :exec aignet-pathcond-rewind$c
+                                      :protect t))))
 
 
