books/centaur/fgl/aignet-pathcond-stobj.lisp
@@ -1,0 +1,331 @@
+; GL - A Symbolic Simulation Framework for ACL2
+; Copyright (C) 2008-2013 Centaur Technology
+;
+; Contact:
+;   Centaur Technology Formal Verification Group
+;   7600-C N. Capital of Texas Highway, Suite 300, Austin, TX 78731, USA.
+;   http://www.centtech.com/
+;
+; License: (An MIT/X11-style license)
+;
+;   Permission is hereby granted, free of charge, to any person obtaining a
+;   copy of this software and associated documentation files (the "Software"),
+;   to deal in the Software without restriction, including without limitation
+;   the rights to use, copy, modify, merge, publish, distribute, sublicense,
+;   and/or sell copies of the Software, and to permit persons to whom the
+;   Software is furnished to do so, subject to the following conditions:
+;
+;   The above copyright notice and this permission notice shall be included in
+;   all copies or substantial portions of the Software.
+;
+;   THE SOFTWARE IS PROVIDED "AS IS", WITHOUT WARRANTY OF ANY KIND, EXPRESS OR
+;   IMPLIED, INCLUDING BUT NOT LIMITED TO THE WARRANTIES OF MERCHANTABILITY,
+;   FITNESS FOR A PARTICULAR PURPOSE AND NONINFRINGEMENT. IN NO EVENT SHALL THE
+;   AUTHORS OR COPYRIGHT HOLDERS BE LIABLE FOR ANY CLAIM, DAMAGES OR OTHER
+;   LIABILITY, WHETHER IN AN ACTION OF CONTRACT, TORT OR OTHERWISE, ARISING
+;   FROM, OUT OF OR IN CONNECTION WITH THE SOFTWARE OR THE USE OR OTHER
+;   DEALINGS IN THE SOFTWARE.
+;
+; Original author: Sol Swords <sswords@centtech.com>
+ 
+(in-package "AIGNET")
+
+(include-book "centaur/aignet/mark-impls" :dir :system)
+(include-book "centaur/misc/intstack" :dir :system)
+(include-book "centaur/fty/baselists" :dir :system)
+(local (include-book "theory"))
+(local (std::add-default-post-define-hook :fix))
+
+
+
+(fty::defalist nbalist :pred nbalistp :key-type natp :val-type bitp :true-listp t :unique-keys t)
+
+
+(local (defthm cdr-hons-assoc-equal-when-nbalistp
+         (implies (nbalistp x)
+                  (and (iff (cdr (hons-assoc-equal n x))
+                            (hons-assoc-equal n x))
+                       (iff (bitp (cdr (hons-assoc-equal n x)))
+                            (hons-assoc-equal n x))))))
+
+
+(defstobj nbalist-stobj$c
+  (nbalist-bits$c :type bitarr)
+  (nbalist-stack$c :type acl2::intstack))
+
+(define nbalist-stobj-to-nbalist-aux ((stack acl2::intstack$ap)
+                                      (bits bit-listp))
+  :returns (nbalist)
+  (if (atom stack)
+      nil
+    (cons (cons (nfix (car stack)) (bfix (nth (car stack) bits)))
+          (nbalist-stobj-to-nbalist-aux (cdr stack) bits)))
+  ///
+  (defret lookup-in-nbalist-stobj-to-nbalist-aux
+    (equal (hons-assoc-equal key nbalist)
+           (and (natp key)
+                (member key (acl2::nat-list-fix stack))
+                (cons key (bfix (nth key bits))))))
+
+  (defret nbalistp-of-nbalist-stobj-to-nbalist-aux
+    (implies (no-duplicatesp-equal (acl2::nat-list-fix stack))
+             (nbalistp nbalist)))
+  
+  (defret len-of-<fn>
+    (equal (len nbalist)
+           (len stack)))
+
+  (local (defthm nth-of-bit-list-fix
+           (bit-equiv (nth n (bit-list-fix x))
+                      (nth n x))
+           :hints(("Goal" :in-theory (enable nth)))))
+
+  (defthm nbalist-stobj-to-nbalist-aux-of-update-non-member
+    (implies (not (member-equal (nfix n) (acl2::nat-list-fix stack)))
+             (equal (nbalist-stobj-to-nbalist-aux stack (update-nth n val bits))
+                    (nbalist-stobj-to-nbalist-aux stack bits))))
+
+  (defthm nbalist-stobj-to-nbalist-aux-of-resize-bits
+    (implies (<= (len bits) (nfix n))
+             (equal (nbalist-stobj-to-nbalist-aux stack (resize-list bits n 0))
+                    (nbalist-stobj-to-nbalist-aux stack bits))))
+
+  (defthm nbalist-stobj-to-nbalist-aux-of-nat-list-fix
+    (equal (nbalist-stobj-to-nbalist-aux (acl2::nat-list-fix stack) bits)
+           (nbalist-stobj-to-nbalist-aux stack bits))
+    :hints(("Goal" :in-theory (enable acl2::nat-list-fix)))))
+
+
+
+(local (defthm nat-listp-when-u32-listp
+         (implies (acl2::u32-listp x)
+                  (nat-listp x))))
+
+(define nbalist-stobj-to-nbalist (nbalist-stobj$c)
+  :non-executable t
+  :returns (nbalist)
+  (nbalist-stobj-to-nbalist-aux (nth *nbalist-stack$c* nbalist-stobj$c)
+                                (nth *nbalist-bits$c* nbalist-stobj$c))
+  ///
+  (defret lookup-in-nbalist-stobj-to-nbalist
+    (equal (hons-assoc-equal key nbalist)
+           (and (natp key)
+                (member key (acl2::nat-list-fix (nth *nbalist-stack$c* nbalist-stobj$c)))
+                (cons key (bfix (nth key (nth *nbalist-bits$c* nbalist-stobj$c)))))))
+
+  (defret nbalistp-of-nbalist-stobj-to-nbalist
+    (implies (nbalist-stobj$cp nbalist-stobj$c)
+             (nbalistp nbalist)))
+  
+  (defret len-of-<fn>
+    (implies (nbalist-stobj$cp nbalist-stobj$c)
+             (equal (len nbalist)
+                    (len (nth *nbalist-stack$c* nbalist-stobj$c))))))
+
+(defun-sk nbalist-stobj$c-size-ok (nbalist-stobj$c)
+  (forall id
+          (implies (member id (acl2::nat-list-fix (nth *nbalist-stack$c* nbalist-stobj$c)))
+                   (< id (len (nth *nbalist-bits$c* nbalist-stobj$c)))))
+  :rewrite :direct)
+
+(in-theory (disable nbalist-stobj$c-size-ok
+                    nbalist-stobj$c-size-ok-necc))
+(local (in-theory (enable nbalist-stobj$c-size-ok-necc)))
+
+(define nbalist-len$c (nbalist-stobj$c)
+  :returns (len natp :rule-classes :type-prescription)
+  :enabled t
+  (mbe :logic (len (nbalist-stobj-to-nbalist nbalist-stobj$c))
+       :exec (stobj-let ((acl2::intstack (nbalist-stack$c nbalist-stobj$c)))
+                        (len)
+                        (acl2::intstack-count acl2::intstack)
+                        len)))
+
+
+(define nbalist-lookup$c ((id natp :type (unsigned-byte 32))
+                          nbalist-stobj$c)
+  :guard (non-exec (ec-call (nbalist-stobj$c-size-ok nbalist-stobj$c)))
+  :returns (ans acl2::maybe-bitp :rule-classes :type-prescription)
+  (mbe :logic (cdr (hons-assoc-equal (nfix id)
+                                     (nbalist-stobj-to-nbalist nbalist-stobj$c)))
+       :exec (stobj-let ((acl2::intstack (nbalist-stack$c nbalist-stobj$c))
+                         (bitarr (nbalist-bits$c nbalist-stobj$c)))
+                        (ans)
+                        (and (acl2::intstack-member^ id acl2::intstack)
+                             (get-bit id bitarr))
+                        ans)))
+
+(define nbalist-push$c ((id natp :type (unsigned-byte 32))
+                        (val bitp)
+                        nbalist-stobj$c)
+  :guard (and (non-exec (ec-call (nbalist-stobj$c-size-ok nbalist-stobj$c)))
+              (not (nbalist-lookup$c id nbalist-stobj$c)))
+  :returns (new-nbalist-stobj$c)
+  (mbe :logic (if (nbalist-lookup$c id nbalist-stobj$c)
+                  nbalist-stobj$c
+                (stobj-let ((acl2::intstack (nbalist-stack$c nbalist-stobj$c))
+                            (bitarr (nbalist-bits$c nbalist-stobj$c)))
+                           (acl2::intstack bitarr)
+                           (b* ((acl2::intstack (non-exec (acl2::nat-list-fix acl2::intstack)))
+                                (acl2::intstack (acl2::intstack-push^ id acl2::intstack))
+                                (bitarr (if (< (nfix id) (bits-length bitarr))
+                                            bitarr
+                                          (resize-bits (max 16 (* 2 (nfix id))) bitarr)))
+                                (bitarr (set-bit id val bitarr)))
+                             (mv acl2::intstack bitarr))
+                           nbalist-stobj$c))
+       :exec (stobj-let ((acl2::intstack (nbalist-stack$c nbalist-stobj$c))
+                         (bitarr (nbalist-bits$c nbalist-stobj$c)))
+                        (acl2::intstack bitarr)
+                        (b* ((acl2::intstack (acl2::intstack-push^ id acl2::intstack))
+                             (bitarr (if (< id (bits-length bitarr))
+                                         bitarr
+                                       (resize-bits (max 16 (* 2 id)) bitarr)))
+                             (bitarr (set-bit id val bitarr)))
+                          (mv acl2::intstack bitarr))
+                        nbalist-stobj$c))
+  ///
+
+  (defret nbalist-stobj-to-nbalist-of-nbalist-push$c
+    (equal (nbalist-stobj-to-nbalist new-nbalist-stobj$c)
+           (b* ((old-nbalist (nbalist-stobj-to-nbalist nbalist-stobj$c)))
+             (if (hons-assoc-equal (nfix id) old-nbalist)
+                 old-nbalist
+               (cons (cons (nfix id) (bfix val)) old-nbalist))))
+    :hints(("Goal" :in-theory (enable nbalist-stobj-to-nbalist
+                                      nbalist-stobj-to-nbalist-aux
+                                      nbalist-lookup$c))))
+
+  (defret nbalist-stobj$c-size-ok-of-<fn>
+    (implies (nbalist-stobj$c-size-ok nbalist-stobj$c)
+             (nbalist-stobj$c-size-ok new-nbalist-stobj$c))
+    :hints ((and stable-under-simplificationp
+                 (let ((lit (assoc 'nbalist-stobj$c-size-ok clause)))
+                   `(:expand (,lit)
+                     :use ((:instance nbalist-stobj$c-size-ok-necc
+                            (id (nbalist-stobj$c-size-ok-witness . ,(cdr lit)))))
+                     :in-theory (disable nbalist-stobj$c-size-ok-necc)))))))
+
+(define nbalist-pop$c (nbalist-stobj$c)
+  :guard (not (equal 0 (nbalist-len$c nbalist-stobj$c)))
+  :returns new-nbalist-stobj$c
+  (stobj-let ((acl2::intstack (nbalist-stack$c nbalist-stobj$c)))
+             (acl2::intstack)
+             (acl2::intstack-pop acl2::intstack)
+             nbalist-stobj$c)
+  ///
+  (defret nbalist-stobj-to-nbalist-of-nbalist-pop$c
+    (equal (nbalist-stobj-to-nbalist new-nbalist-stobj$c)
+           (cdr (nbalist-stobj-to-nbalist nbalist-stobj$c)))
+    :hints(("Goal" :in-theory (enable nbalist-stobj-to-nbalist
+                                      nbalist-stobj-to-nbalist-aux))))
+
+  (defret nbalist-stobj$c-size-ok-of-<fn>
+    (implies (nbalist-stobj$c-size-ok nbalist-stobj$c)
+             (nbalist-stobj$c-size-ok new-nbalist-stobj$c))
+    :hints ((and stable-under-simplificationp
+                 (let ((lit (assoc 'nbalist-stobj$c-size-ok clause)))
+                   `(:computed-hint-replacement
+                     ((and stable-under-simplificationp
+                           '(:in-theory (enable acl2::nat-list-fix))))
+                     :expand (,lit)
+                     :use ((:instance nbalist-stobj$c-size-ok-necc
+                            (id (nbalist-stobj$c-size-ok-witness . ,(cdr lit)))))
+                     :in-theory (e/d ()
+                                     (nbalist-stobj$c-size-ok-necc))))))))
+
+(define nbalist-stobj$ap (nbalist)
+  :enabled t
+  (nbalistp nbalist))
+
+(define create-nbalist-stobj$a () nil)
+
+(define nbalist-stobj-len$a ((nbalist nbalist-stobj$ap))
+  :enabled t
+  (len (nbalist-fix nbalist)))
+
+(define nbalist-lookup ((id natp)
+                        (nbalist nbalistp))
+  :returns ans
+  (cdr (hons-get (nfix id) (nbalist-fix nbalist))))
+
+(local (in-theory (enable nbalist-lookup)))
+
+(define nbalist-stobj-lookup$a ((id (unsigned-byte-p 32 id))
+                                (nbalist nbalist-stobj$ap))
+  :enabled t
+  (nbalist-lookup id nbalist))
+
+(define nbalist-stobj-push$a ((id (unsigned-byte-p 32 id))
+                              (val bitp)
+                              (nbalist nbalist-stobj$ap))
+  :guard (not (nbalist-stobj-lookup$a id nbalist))
+  :enabled t
+  (nbalist-fix (cons (cons id val) nbalist)))
+
+(define nbalist-stobj-pop$a ((nbalist nbalist-stobj$ap))
+  :enabled t
+  :guard (not (equal 0 (nbalist-stobj-len$a nbalist)))
+  :prepwork ((local (in-theory (enable nbalistp))))
+  (cdr (nbalist-fix nbalist)))
+
+
+  
+
+
+(encapsulate nil
+  (local
+   (define nbalist-stobj-corr (nbalist-stobj$c nbalist)
+     :enabled t
+     :verify-guards nil
+     (and (equal nbalist (nbalist-stobj-to-nbalist nbalist-stobj$c))
+          (nbalist-stobj$c-size-ok nbalist-stobj$c))))
+
+  (local (defthm nbalist-stobj$c-size-ok-of-empty
+           (nbalist-stobj$c-size-ok '(nil nil))
+           :hints(("Goal" :in-theory (enable nbalist-stobj$c-size-ok)))))
+
+  (local (defthm nbalist-stobj-to-nbalist-of-empty
+           (not (nbalist-stobj-to-nbalist '(nil nil)))
+           :hints(("Goal" :in-theory (e/d (nbalist-stobj-to-nbalist)
+                                          ((nbalist-stobj-to-nbalist)))))))
+
+  (local (in-theory (enable nbalist-lookup$c)))
+
+  (defabsstobj-events nbalist-stobj
+    :concrete nbalist-stobj$c
+    :corr-fn nbalist-stobj-corr
+    :recognizer (nbalist-stobjp :logic nbalist-stobj$ap
+                               :exec nbalist-stobj$cp)
+    :creator (create-nbalist-stobj :logic create-nbalist-stobj$a
+                                  :exec create-nbalist-stobj$c)
+    :exports ((nbalist-stobj-lookup^ :logic nbalist-stobj-lookup$a
+                                   :exec nbalist-lookup$c)
+              (nbalist-stobj-len :logic nbalist-stobj-len$a
+                                :exec nbalist-len$c)
+              (nbalist-stobj-push^ :logic nbalist-stobj-push$a
+                                  :exec nbalist-push$c
+                                  :protect t)
+              (nbalist-stobj-pop :logic nbalist-stobj-pop$a
+                                :exec nbalist-pop$c
+                                :protect t))))
+  
+
+(define nbalist-stobj-lookup ((id natp)
+                              nbalist-stobj)
+  :enabled t
+  (mbe :logic (non-exec (nbalist-lookup id nbalist-stobj))
+       :exec (if (<= id #xfffffff)
+                 (nbalist-stobj-lookup^ id nbalist-stobj)
+               (ec-call (nbalist-stobj-lookup^ id nbalist-stobj)))))
+
+(define nbalist-stobj-push ((id natp)
+                            (val bitp)
+                            nbalist-stobj)
+  :enabled t
+  :guard (not (nbalist-stobj-lookup id nbalist-stobj))
+  (mbe :logic (non-exec (nbalist-fix (cons (cons id val) nbalist-stobj)))
+       :exec (if (<= id #xfffffff)
+                 (nbalist-stobj-push^ id val nbalist-stobj)
+               (ec-call (nbalist-stobj-push^ id val nbalist-stobj)))))
+
