books/centaur/fgl/pathcond-base.lisp
@@ -1,0 +1,218 @@
+; GL - A Symbolic Simulation Framework for ACL2
+; Copyright (C) 2008-2013 Centaur Technology
+;
+; Contact:
+;   Centaur Technology Formal Verification Group
+;   7600-C N. Capital of Texas Highway, Suite 300, Austin, TX 78731, USA.
+;   http://www.centtech.com/
+;
+; License: (An MIT/X11-style license)
+;
+;   Permission is hereby granted, free of charge, to any person obtaining a
+;   copy of this software and associated documentation files (the "Software"),
+;   to deal in the Software without restriction, including without limitation
+;   the rights to use, copy, modify, merge, publish, distribute, sublicense,
+;   and/or sell copies of the Software, and to permit persons to whom the
+;   Software is furnished to do so, subject to the following conditions:
+;
+;   The above copyright notice and this permission notice shall be included in
+;   all copies or substantial portions of the Software.
+;
+;   THE SOFTWARE IS PROVIDED "AS IS", WITHOUT WARRANTY OF ANY KIND, EXPRESS OR
+;   IMPLIED, INCLUDING BUT NOT LIMITED TO THE WARRANTIES OF MERCHANTABILITY,
+;   FITNESS FOR A PARTICULAR PURPOSE AND NONINFRINGEMENT. IN NO EVENT SHALL THE
+;   AUTHORS OR COPYRIGHT HOLDERS BE LIABLE FOR ANY CLAIM, DAMAGES OR OTHER
+;   LIABILITY, WHETHER IN AN ACTION OF CONTRACT, TORT OR OTHERWISE, ARISING
+;   FROM, OUT OF OR IN CONNECTION WITH THE SOFTWARE OR THE USE OR OTHER
+;   DEALINGS IN THE SOFTWARE.
+;
+; Original author: Sol Swords <sswords@centtech.com>
+ 
+(in-package "FGL")
+
+(include-book "pathcond-aig")
+(include-book "pathcond-aignet")
+(include-book "pathcond-stobj")
+
+(local (include-book "theory"))
+
+
+
+(defsection pathcondp
+  (local (in-theory (enable pathcondp)))
+  (defthm pathcondp-implies-ubddp
+    (implies (pathcondp x)
+             (acl2::ubddp (nth *pathcond-bdd* x))))
+
+  (defthm pathcondp-implies-calistp
+    (implies (pathcondp x)
+             (calistp (nth *pathcond-aig* x))))
+
+  (defthm pathcondp-implies-nbalistp
+    (implies (pathcondp x)
+             (aignet::nbalistp (nth *pathcond-aignet* x))))
+
+  (local (in-theory (enable aignet::redundant-update-nth)))
+
+  (defthm pathcondp-implies-update-bdd-equal
+    (implies (and (pathcondp x)
+                  (equal bdd (nth *pathcond-bdd* x)))
+             (equal (update-nth *pathcond-bdd* bdd x) x)))
+
+  (defthm pathcondp-implies-update-aig-equal
+    (implies (and (pathcondp x)
+                  (equal calist (nth *pathcond-aig* x)))
+             (equal (update-nth *pathcond-aig* calist x) x)))
+
+  (defthm pathcondp-implies-update-aignet-equal
+    (implies (and (pathcondp x)
+                  (equal nbalist (nth *pathcond-aignet* x)))
+             (equal (update-nth *pathcond-aignet* nbalist x) x)))
+
+  (defthm pathcondp-of-update-bdd
+    (implies (and (pathcondp x)
+                  (acl2::ubddp bdd))
+             (pathcondp (update-nth *pathcond-bdd* bdd x))))
+
+  (defthm pathcondp-of-update-aig
+    (implies (and (pathcondp x)
+                  (calistp calist))
+             (pathcondp (update-nth *pathcond-aig* calist x))))
+
+  (defthm pathcondp-of-update-aignet
+    (implies (and (pathcondp x)
+                  (aignet::nbalistp nbalist))
+             (pathcondp (update-nth *pathcond-aignet* nbalist x)))))
+
+(define pathcond-fix (pathcond)
+  :returns (new-pathcond pathcondp)
+  :guard-hints (("goal" :expand ((len pathcond)
+                                 (len (cdr pathcond))
+                                 (len (cddr pathcond)))))
+  (mbe :logic (non-exec (list (acl2::ubdd-fix (pathcond-bdd pathcond))
+                              (calist-fix (pathcond-aig pathcond))
+                              (aignet::nbalist-fix (pathcond-aignet pathcond))))
+       :exec pathcond)
+  ///
+  (defthm nth-of-pathcond-fix
+    (and (equal (nth *pathcond-bdd* (pathcond-fix pathcond))
+                (acl2::ubdd-fix (nth *pathcond-bdd* pathcond)))
+         (equal (nth *pathcond-aig* (pathcond-fix pathcond))
+                (calist-fix (nth *pathcond-aig* pathcond)))
+         (equal (nth *pathcond-aignet* (pathcond-fix pathcond))
+                (aignet::nbalist-fix (nth *pathcond-aignet* pathcond)))))
+
+  (local (defthm equal-of-cons
+           (equal (equal (cons a b) c)
+                  (and (consp c)
+                       (equal (car c) a)
+                       (equal (cdr c) b)))))
+
+  (defthm pathcond-fix-when-pathcondp
+    (implies (pathcondp pathcond)
+             (equal (pathcond-fix pathcond) pathcond))
+    :hints (("goal" :expand ((len pathcond)
+                             (len (cdr pathcond))
+                             (len (cddr pathcond))
+                             (len (cdddr pathcond))))))
+
+  (defun-nx pathcond-equiv (x y)
+    (equal (pathcond-fix x) (pathcond-fix y)))
+
+  (defequiv pathcond-equiv)
+
+  (fty::deffixtype pathcond :pred pathcondp :fix pathcond-fix :equiv pathcond-equiv)
+
+  (in-theory (disable pathcondp)))
+
+(define pathcond-checkpoint-p (x (bfr-mode bfr-mode-p) pathcond)
+  (bfr-mode-case
+    :aig (and (natp x)
+              (stobj-let ((calist-stobj (pathcond-aig pathcond)))
+                         (ok)
+                         (<= x (calist-stobj-len calist-stobj))
+                         ok))
+    :aignet (and (natp x)
+                 (stobj-let ((aignet-pathcond (pathcond-aignet pathcond)))
+                            (ok)
+                            (<= x (aignet-pathcond-len aignet-pathcond))
+                            ok))
+    :bdd (acl2::ubddp x)))
+
+(define pathcond-checkpoint ((bfr-mode bfr-mode-p) pathcond)
+  :returns (chp (pathcond-checkpoint-p chp bfr-mode pathcond)
+                :hints(("Goal" :in-theory (enable pathcond-checkpoint-p))))
+  (bfr-mode-case
+    :bdd (mbe :logic (acl2::ubdd-fix (pathcond-bdd pathcond))
+              :exec (pathcond-bdd pathcond))
+    :aig (stobj-let ((calist-stobj (pathcond-aig pathcond)))
+                    (len)
+                    (calist-stobj-len calist-stobj)
+                    len)
+    :aignet (stobj-let ((aignet-pathcond (pathcond-aignet pathcond)))
+                       (len)
+                       (aignet-pathcond-len aignet-pathcond)
+                       len)))
+
+(define pathcond-rewindable ((bfr-mode bfr-mode-p) (new pathcondp) (old pathcondp))
+  :verify-guards nil
+  :non-executable t
+  (b* ((new (pathcond-fix new))
+       (old (pathcond-fix old)))
+    (bfr-mode-case
+      :aig (and (equal new (update-nth *pathcond-aig* (nth *pathcond-aig* new) old))
+                (calist-extension-p (nth *pathcond-aig* new) (nth *pathcond-aig* old)))
+      :aignet (and (equal new (update-nth *pathcond-aignet* (nth *pathcond-aignet* new) old))
+                   (aignet::nbalist-extension-p (nth *pathcond-aignet* new) (nth *pathcond-aignet* old)))
+      :bdd (equal new (update-nth *pathcond-bdd* (nth *pathcond-bdd* new) old))))
+  ///
+  (defthm pathcond-checkpoint-p-when-rewindable
+    (implies (and (pathcond-rewindable bfr-mode new old)
+                  (pathcond-checkpoint-p chp bfr-mode old))
+             (pathcond-checkpoint-p chp bfr-mode new))
+    :hints(("Goal" :in-theory (enable pathcond-checkpoint-p))))
+
+  (defthm pathcond-rewindable-of-self
+    (pathcond-rewindable bfr-mode x x)
+    :hints(("Goal" :in-theory (enable aignet::nbalist-extension-p
+                                      calist-extension-p)))))
+
+(define pathcond-rewind ((chp (pathcond-checkpoint-p chp bfr-mode pathcond))
+                         (bfr-mode bfr-mode-p)
+                         pathcond)
+  :guard-hints (("goal" :in-theory (enable pathcond-checkpoint-p)))
+  (b* ((pathcond (pathcond-fix pathcond)))
+    (bfr-mode-case
+      :aig (stobj-let ((calist-stobj (pathcond-aig pathcond)))
+                      (calist-stobj)
+                      (rewind-calist chp calist-stobj)
+                      pathcond)
+      :aignet (stobj-let ((aignet-pathcond (pathcond-aignet pathcond)))
+                         (aignet-pathcond)
+                         (aignet-pathcond-rewind chp aignet-pathcond)
+                         pathcond)
+      :bdd (update-pathcond-bdd (acl2::ubdd-fix chp) pathcond)))
+  ///
+  (local (defthm update-nth-same
+           (equal (update-nth n v1 (update-nth n v2 x))
+                  (update-nth n v1 x))
+           :hints(("Goal" :in-theory (enable update-nth)))))
+  (local (defthm update-nth-lemma
+           (implies (equal x (update-nth n val y))
+                    (equal (update-nth n val1 x)
+                           (update-nth n val1 y)))))
+
+  (defthm pathcond-rewind-when-rewindable
+    (implies (pathcond-rewindable bfr-mode new old)
+             (equal (pathcond-rewind (pathcond-checkpoint bfr-mode old) bfr-mode new)
+                    (pathcond-fix old)))
+    :hints(("Goal" :in-theory (enable pathcond-rewindable
+                                      pathcond-checkpoint))))
+
+  (defthm pathcond-rewind-when-rewindable-free
+    (implies (and (pathcond-rewindable bfr-mode new old)
+                  (equal (pathcond-checkpoint bfr-mode old) chp))
+             (equal (pathcond-rewind chp bfr-mode new)
+                    (pathcond-fix old)))))
+  
+
