books/centaur/fgl/pathcond-stobj.lisp
@@ -1,0 +1,64 @@
+; GL - A Symbolic Simulation Framework for ACL2
+; Copyright (C) 2008-2013 Centaur Technology
+;
+; Contact:
+;   Centaur Technology Formal Verification Group
+;   7600-C N. Capital of Texas Highway, Suite 300, Austin, TX 78731, USA.
+;   http://www.centtech.com/
+;
+; License: (An MIT/X11-style license)
+;
+;   Permission is hereby granted, free of charge, to any person obtaining a
+;   copy of this software and associated documentation files (the "Software"),
+;   to deal in the Software without restriction, including without limitation
+;   the rights to use, copy, modify, merge, publish, distribute, sublicense,
+;   and/or sell copies of the Software, and to permit persons to whom the
+;   Software is furnished to do so, subject to the following conditions:
+;
+;   The above copyright notice and this permission notice shall be included in
+;   all copies or substantial portions of the Software.
+;
+;   THE SOFTWARE IS PROVIDED "AS IS", WITHOUT WARRANTY OF ANY KIND, EXPRESS OR
+;   IMPLIED, INCLUDING BUT NOT LIMITED TO THE WARRANTIES OF MERCHANTABILITY,
+;   FITNESS FOR A PARTICULAR PURPOSE AND NONINFRINGEMENT. IN NO EVENT SHALL THE
+;   AUTHORS OR COPYRIGHT HOLDERS BE LIABLE FOR ANY CLAIM, DAMAGES OR OTHER
+;   LIABILITY, WHETHER IN AN ACTION OF CONTRACT, TORT OR OTHERWISE, ARISING
+;   FROM, OUT OF OR IN CONNECTION WITH THE SOFTWARE OR THE USE OR OTHER
+;   DEALINGS IN THE SOFTWARE.
+;
+; Original author: Sol Swords <sswords@centtech.com>
+ 
+(in-package "FGL")
+
+(include-book "pathcond-aignet")
+(include-book "aig-pathcond-stobj")
+(include-book "centaur/ubdds/lite" :dir :system)
+
+(acl2::defstobj-clone aignet-pathcond aignet::aignet-pathcond
+  :strsubst (("abcd" . "abcd")) :pkg gl-package)
+
+(defstobj pathcond
+  (pathcond-bdd :type (satisfies acl2::ubddp) :initially t)
+  (pathcond-aig :type calist-stobj)
+  (pathcond-aignet :type aignet-pathcond))
+
+(std::defenum bfr-mode-p
+  (t nil :aignet))
+
+(defsection bfr-mode-case
+  :short "Choose behavior based on a bfr-mode object"
+  :long "<p>Usage:</p>
+
+@({
+     (bfr-mode-case :aig aig-code
+                    :bdd bdd-code
+                    :aignet aignet-code)
+})
+
+@(def bfr-mode-case)"
+
+  (defmacro bfr-mode-case (&key aig bdd aignet)
+    `(case (bfr-mode-fix bfr-mode)
+       ((nil) ,bdd)
+       (:aignet ,aignet)
+       (t ,aig))))
