books/centaur/fgl/pathcond.lisp
@@ -1,0 +1,396 @@
+; GL - A Symbolic Simulation Framework for ACL2
+; Copyright (C) 2018 Centaur Technology
+;
+; Contact:
+;   Centaur Technology Formal Verification Group
+;   7600-C N. Capital of Texas Highway, Suite 300, Austin, TX 78731, USA.
+;   http://www.centtech.com/
+;
+; License: (An MIT/X11-style license)
+;
+;   Permission is hereby granted, free of charge, to any person obtaining a
+;   copy of this software and associated documentation files (the "Software"),
+;   to deal in the Software without restriction, including without limitation
+;   the rights to use, copy, modify, merge, publish, distribute, sublicense,
+;   and/or sell copies of the Software, and to permit persons to whom the
+;   Software is furnished to do so, subject to the following conditions:
+;
+;   The above copyright notice and this permission notice shall be included in
+;   all copies or substantial portions of the Software.
+;
+;   THE SOFTWARE IS PROVIDED "AS IS", WITHOUT WARRANTY OF ANY KIND, EXPRESS OR
+;   IMPLIED, INCLUDING BUT NOT LIMITED TO THE WARRANTIES OF MERCHANTABILITY,
+;   FITNESS FOR A PARTICULAR PURPOSE AND NONINFRINGEMENT. IN NO EVENT SHALL THE
+;   AUTHORS OR COPYRIGHT HOLDERS BE LIABLE FOR ANY CLAIM, DAMAGES OR OTHER
+;   LIABILITY, WHETHER IN AN ACTION OF CONTRACT, TORT OR OTHERWISE, ARISING
+;   FROM, OUT OF OR IN CONNECTION WITH THE SOFTWARE OR THE USE OR OTHER
+;   DEALINGS IN THE SOFTWARE.
+;
+; Original author: Sol Swords <sswords@centtech.com>
+
+(in-package "FGL")
+
+(include-book "logicman")
+(include-book "pathcond-base")
+(local (include-book "theory"))
+(local (include-book "tools/trivial-ancestors-check" :dir :system))
+
+(define logicman-pathcond-checkpoint-p (x &optional (logicman 'logicman))
+  :enabled t
+  (b* ((bfr-mode (bfr-mode)))
+    (stobj-let ((pathcond (logicman->pathcond logicman)))
+               (ok)
+               (pathcond-checkpoint-p x bfr-mode pathcond)
+               ok))
+  ;; ///
+  ;; (def-updater-independence-thm logicman-pathcond-checkpoint-p-updater-independence
+  ;;   (implies (and (equal (logicman->pathcond new)
+  ;;                        (logicman->pathcond old))
+  ;;                 (equal (logicman->mode new)
+  ;;                        (logicman->mode old)))
+  ;;            (equal (logicman-pathcond-checkpoint-p x new)
+  ;;                   (logicman-pathcond-checkpoint-p x old))))
+  )
+
+(define logicman-pathcond-checkpoint (&optional (logicman 'logicman))
+  :enabled t
+  (b* ((bfr-mode (bfr-mode)))
+    (stobj-let ((pathcond (logicman->pathcond logicman)))
+               (chp)
+               (pathcond-checkpoint bfr-mode pathcond)
+               chp))
+  ;; ///
+  ;; (def-updater-independence-thm logicman-pathcond-checkpoint-updater-independence
+  ;;   (implies (and (equal (logicman->pathcond new)
+  ;;                        (logicman->pathcond old))
+  ;;                 (equal (logicman->mode new)
+  ;;                        (logicman->mode old)))
+  ;;            (equal (logicman-pathcond-checkpoint new)
+  ;;                   (logicman-pathcond-checkpoint old))))
+  )
+
+(define logicman-pathcond-rewindable (new old)
+  :non-executable t
+  :verify-guards nil
+  :enabled t
+  (b* ((bfr-mode (bfr-mode old)))
+    (and (equal (bfr-mode new) bfr-mode)
+         (pathcond-rewindable bfr-mode (logicman->pathcond new) (logicman->pathcond old))))
+  ;; ///
+  ;; (defthm logicman-pathcond-checkpoint-p-when-rewindable
+  ;;   (implies (and (logicman-pathcond-rewindable new old)
+  ;;                 (logicman-pathcond-checkpoint-p chp old))
+  ;;            (logicman-pathcond-checkpoint-p chp new))
+  ;;   :hints(("Goal" :in-theory (enable logicman-pathcond-checkpoint-p))))
+
+  ;; (defthm logicman-pathcond-checkpoint-rewindable-of-self
+  ;;   (logicman-pathcond-rewindable x x))
+
+  ;; (def-updater-independence-thm logicman-pathcond-rewindable-updater-independence
+  ;;   (implies (and (equal (logicman->pathcond new)
+  ;;                        (logicman->pathcond old))
+  ;;                 (equal (logicman->mode new)
+  ;;                        (logicman->mode old)))
+  ;;            (equal (logicman-pathcond-rewindable new x)
+  ;;                   (logicman-pathcond-rewindable old x))))
+  )
+
+(define logicman-pathcond-rewind ((chp logicman-pathcond-checkpoint-p)
+                                  &optional (logicman 'logicman))
+  :returns (new-logicman)
+  :guard-hints (("goal" :in-theory (enable logicman-pathcond-checkpoint-p)))
+  (b* ((bfr-mode (bfr-mode)))
+    (stobj-let ((pathcond (logicman->pathcond logicman)))
+               (pathcond)
+               (pathcond-rewind chp bfr-mode pathcond)
+               logicman))
+  ///
+  (defret logicman-get-of-logicman-pathcond-rewind
+    (implies (not (equal (logicman-field-fix key) :pathcond))
+             (equal (logicman-get key new-logicman)
+                    (logicman-get key logicman))))
+
+  (defret logicman-extension-p-of-logicman-pathcond-rewind
+    (logicman-extension-p new-logicman logicman))
+
+  (defthm logicman-pathcond-rewind-when-rewindable
+    (implies (and (logicman-pathcond-rewindable new old)
+                  (equal bfr-mode (logicman->mode old)))
+             (equal (logicman->pathcond (logicman-pathcond-rewind
+                                         (pathcond-checkpoint bfr-mode (logicman->pathcond old))
+                                         new))
+                    (pathcond-fix (logicman->pathcond old))))))
+
+(local (defthm bitp-when-maybe-bitp
+         (implies (and x (acl2::maybe-bitp x))
+                  (bitp x))))
+
+
+(define logicman-pathcond-eval (env &optional (logicman 'logicman))
+  (declare (xargs :non-executable t))
+  :no-function t
+  :verify-guards nil
+  (prog2$ (acl2::throw-nonexec-error 'logicman-pathcond-eval-fn (list env logicman))
+          (bfr-case
+            :bdd (b* ((pathcond-bdd (stobj-let ((pathcond (logicman->pathcond logicman)))
+                                               (bdd)
+                                               (pathcond-bdd pathcond)
+                                               (bfr-fix bdd))))
+                   (bfr-eval pathcond-bdd env))
+            :aig (stobj-let ((pathcond (logicman->pathcond logicman)))
+                            (ans)
+                            (stobj-let ((calist-stobj (pathcond-aig pathcond)))
+                                       (ans)
+                                       (calist-eval calist-stobj env)
+                                       ans)
+                            ans)
+            :aignet (stobj-let ((pathcond (logicman->pathcond logicman))
+                                (aignet   (logicman->aignet logicman)))
+                               (ans)
+                               (stobj-let ((aignet-pathcond (pathcond-aignet pathcond)))
+                                          (ans)
+                                          (aignet::aignet-pathcond-eval
+                                           aignet aignet-pathcond
+                                           (alist-to-bitarr (aignet::num-ins aignet) env nil)
+                                           nil)
+                                          ans)
+                               ans))))
+                                  
+
+
+(define logicman-pathcond-implies-aignet-base ((x bfr-p)
+                                               &optional (logicman 'logicman))
+  :prepwork ((local (in-theory (enable bfr->aignet-lit bfr-p aignet::aignet-idp))))
+  :guard (eq (bfr-mode) :aignet)
+  :enabled t
+  (b* ((lit (bfr->aignet-lit x)))
+    (stobj-let ((pathcond (logicman->pathcond logicman))
+                (aignet   (logicman->aignet logicman)))
+               (ans pathcond)
+               (stobj-let ((aignet-pathcond (pathcond-aignet pathcond)))
+                          (ans aignet-pathcond)
+                          (aignet-pathcond-implies (aignet::lit->var lit) aignet aignet-pathcond)
+                          (mv (and ans (b-xor (aignet::lit->neg lit) ans)) pathcond))
+               (mv ans logicman))))
+
+(define logicman-pathcond-implies ((x bfr-p)
+                                   &optional (logicman 'logicman))
+  :returns (mv (ans acl2::maybe-bitp :rule-classes :type-prescription)
+               (new-logicman (equal new-logicman logicman)))
+  :guard-hints ((and stable-under-simplificationp
+                     '(:in-theory (enable bfr-p))))
+  :prepwork ((local (in-theory (disable (force)))))
+  (b* ((x (bfr-fix x)))
+    (bfr-case
+      :bdd (b* ((pathcond-bdd (stobj-let ((pathcond (logicman->pathcond logicman)))
+                                         (bdd)
+                                         (pathcond-bdd pathcond)
+                                         (mbe :logic (acl2::ubdd-fix bdd) :exec bdd)))
+                ((when (acl2::q-and-is-nil pathcond-bdd x)) (mv 0 logicman))
+                ((when (acl2::q-and-is-nilc2 pathcond-bdd x)) (mv 1 logicman)))
+             (mv nil logicman))
+      :aig (stobj-let ((pathcond (logicman->pathcond logicman)))
+                      (ans)
+                      (stobj-let ((calist-stobj (pathcond-aig pathcond)))
+                                 (ans)
+                                 (calist-implies x (calist-stobj-access calist-stobj))
+                                 ans)
+                      (mv ans logicman))
+      :aignet (mbe :logic (non-exec
+                           (b* (((mv ans ?new-logicman)
+                                 (logicman-pathcond-implies-aignet-base x)))
+                             (mv ans logicman)))
+                   :exec (logicman-pathcond-implies-aignet-base x))))
+  ///
+  ;; (local (defthm backchaining-hack
+  ;;          (implies (not (equal (aignet::aignet-pathcond-implies-logic x aignet pathcond) b))
+  ;;                   (not (equal (aignet::aignet-pathcond-implies-logic x aignet pathcond) b)))))
+  ;; (local (acl2::use-trivial-ancestors-check))
+
+  (defret eval-when-logicman-pathcond-implies
+    (implies (and (logicman-pathcond-eval env)
+                  ans)
+             (equal ans (bool->bit (bfr-eval x env))))
+    :hints(("Goal" :in-theory (enable logicman-pathcond-eval bfr-eval bfr-fix bfr->aignet-lit aignet-lit->bfr
+                                      aignet::lit-eval-of-aignet-lit-fix
+                                      aignet::aignet-lit-fix aignet::aignet-id-fix
+                                      aignet::aignet-idp)
+            :expand ((:free (invals regvals aignet) (aignet::lit-eval x invals regvals aignet)))
+            :do-not-induct t)
+           (and stable-under-simplificationp
+                (let ((lit (assoc 'acl2::q-binary-and clause)))
+                  (and lit
+                       `(:use ((:instance acl2::eval-bdd-of-q-and
+                                (x ,(second lit)) (y ,(third lit))
+                                (values env)))
+                         :in-theory (disable acl2::eval-bdd-of-q-and))))))
+    :otf-flg t)
+
+  (defret logicman-pathcond-implies-not-equal-negation
+    (implies (and (logicman-pathcond-eval env)
+                  (equal b (b-not (bool->bit (bfr-eval x env)))))
+             (not (equal ans b)))
+    :hints (("goal" :use eval-when-logicman-pathcond-implies))))
+
+
+(define logicman-pathcond-depends-on ((v bfr-varname-p)
+                                      &optional ((logicman logicman-nvars-ok) 'logicman))
+  (bfr-case
+    :bdd (stobj-let ((pathcond (logicman->pathcond logicman)))
+                    (dep)
+                    (ec-call (nth v (acl2::ubdd-deps (acl2::ubdd-fix (pathcond-bdd pathcond)))))
+                    dep)
+    :aig (stobj-let ((pathcond (logicman->pathcond logicman)))
+                    (dep)
+                    (stobj-let ((calist-stobj (pathcond-aig pathcond)))
+                               (dep)
+                               (calist-depends-on v (calist-stobj-access calist-stobj))
+                               dep)
+                    dep)
+    :aignet (stobj-let ((pathcond (logicman->pathcond logicman))
+                        (aignet (logicman->aignet logicman)))
+                       (dep)
+                       (stobj-let ((aignet-pathcond (pathcond-aignet pathcond)))
+                                  (dep)
+                                  (non-exec
+                                   (ec-call (aignet::nbalist-depends-on
+                                             v aignet-pathcond aignet)))
+                                  dep)
+                       dep))
+  ///
+
+  (local #!acl2
+         (defthm eval-bdd-of-update-when-not-dependent-fix
+           (implies (not (nth n (ubdd-deps (ubdd-fix x))))
+                    (equal (eval-bdd x (update-nth n v env))
+                           (eval-bdd x env)))
+           :hints (("goal" :use ((:instance eval-bdd-of-update-when-not-dependent
+                                  (x (ubdd-fix x))))
+                    :in-theory (disable eval-bdd-of-update-when-not-dependent)))))
+
+    (local (defthm alist-to-bitarr-of-cons
+           (acl2::bits-equiv (alist-to-bitarr max (cons (cons var val) alist) bitarr)
+                             (if (and (natp var)
+                                      (< var (nfix max)))
+                                 (update-nth var (bool->bit val) (alist-to-bitarr max alist bitarr))
+                               (alist-to-bitarr max alist bitarr)))
+           :hints(("Goal" :in-theory (enable acl2::bits-equiv)))))
+           
+
+  (defthm logicman-pathcond-eval-of-set-var-when-not-depends-on
+    (implies (and (not (logicman-pathcond-depends-on v))
+                  (bfr-varname-p v))
+             (equal (logicman-pathcond-eval (bfr-set-var v val env))
+                    (logicman-pathcond-eval env)))
+    :hints(("Goal" :in-theory (enable logicman-pathcond-eval bfr-eval bfr-fix
+                                      bfr-set-var bfr-varname-p bfr-nvars)))))
+
+
+(define logicman-pathcond-assume ((x bfr-p)
+                                  &optional (logicman 'logicman))
+  :returns (mv contradictionp
+               new-logicman)
+  :guard-hints (("goal" :in-theory (enable bfr-p bfr->aignet-lit aignet::aignet-idp)))
+  (b* ((x (bfr-fix x)))
+    (bfr-case
+      :bdd (stobj-let ((pathcond (logicman->pathcond logicman)))
+                      (contra pathcond)
+                      (b* ((pathcond (pathcond-fix pathcond))
+                           (pathcond-bdd (pathcond-bdd pathcond))
+                           (pathcond-bdd (mbe :logic (acl2::ubdd-fix pathcond-bdd)
+                                              :exec pathcond-bdd))
+                           (new-pathcond-bdd (acl2::q-and pathcond-bdd x))
+                           ((when (eq new-pathcond-bdd nil))
+                            (mv t pathcond))
+                           (pathcond (update-pathcond-bdd new-pathcond-bdd pathcond)))
+                        (mv nil pathcond))
+                      (mv contra logicman))
+      :aig (stobj-let ((pathcond (logicman->pathcond logicman)))
+                      (contra pathcond)
+                      (b* ((pathcond (pathcond-fix pathcond)))
+                        (stobj-let ((calist-stobj (pathcond-aig pathcond)))
+                                   (contra calist-stobj)
+                                   (calist-assume x calist-stobj)
+                                   (mv contra pathcond)))
+                      (mv contra logicman))
+      :aignet (b* ((x (bfr->aignet-lit x)))
+                (stobj-let ((pathcond (logicman->pathcond logicman))
+                            (aignet (logicman->aignet logicman)))
+                           (contra pathcond)
+                           (b* ((pathcond (pathcond-fix pathcond)))
+                             (stobj-let ((aignet-pathcond (pathcond-aignet pathcond)))
+                                        (contra aignet-pathcond)
+                                        (aignet-pathcond-assume x aignet aignet-pathcond)
+                                        (mv contra pathcond)))
+                           (mv contra logicman)))))
+  ///
+  (defret logicman-get-of-logicman-pathcond-assume
+    (implies (not (equal (logicman-field-fix key) :pathcond))
+             (equal (logicman-get key new-logicman)
+                    (logicman-get key logicman))))
+
+  (defret logicman-extension-p-of-logicman-pathcond-assume
+    (logicman-extension-p new-logicman logicman))
+  
+
+  (defret logicman-pathcond-assume-correct
+    (implies (and (logicman-pathcond-eval env)
+                  (bfr-eval x env))
+             (and (not contradictionp)
+                  (logicman-pathcond-eval env new-logicman)))
+    :hints(("Goal" :in-theory (enable bfr-eval bfr-fix bfr-p bfr->aignet-lit
+                                      logicman-pathcond-eval))
+           (and stable-under-simplificationp
+                (let ((lit (assoc 'acl2::q-binary-and clause)))
+                  (and lit
+                       `(:use ((:instance acl2::eval-bdd-of-q-and
+                                (x ,(second lit)) (y ,(third lit))
+                                (values env)))
+                         :in-theory (disable acl2::eval-bdd-of-q-and))))))
+    :otf-flg t)
+
+  (defret logicman-pathcond-assume-eval-new
+    (implies (not contradictionp)
+             (equal (logicman-pathcond-eval env new-logicman)
+                    (and (logicman-pathcond-eval env)
+                         (bfr-eval x env))))
+    :hints(("Goal" :in-theory (enable bfr-eval bfr-fix bfr->aignet-lit logicman-pathcond-eval))))
+
+  (defret logicman-pathcond-assume-contradictionp-correct
+    (implies (and contradictionp
+                  (bfr-eval x env))
+             (not (logicman-pathcond-eval env logicman)))
+    :hints (("goal" :use logicman-pathcond-assume-correct)))
+
+  (local (in-theory (disable (force))))
+
+  (defret pathcond-rewindable-of-logicman-pathcond-assume
+    (implies (equal (bfr-mode-fix bfr-mode) (bfr-mode))
+             (pathcond-rewindable bfr-mode (logicman->pathcond new-logicman)  (logicman->pathcond logicman)))
+    :hints(("Goal" :in-theory (enable pathcond-rewindable bfr-fix))))
+
+  ;; (local
+  ;;  #!aignet
+  ;;  (Defthm depends-on-of-aignet-lit-fix
+  ;;    (equal (depends-on (aignet-lit-fix lit aignet) ci-id aignet)
+  ;;           (depends-on lit ci-id aignet))
+  ;;    :hints (("goal" :expand ((depends-on (aignet-lit-fix lit aignet)
+  ;;                                         ci-id aignet)
+  ;;                             (depends-on lit ci-id aignet))))))
+
+  (defret logicman-pathcond-depends-on-of-logicman-pathcond-assume
+    (implies (and (not (logicman-pathcond-depends-on v))
+                  (not (bfr-depends-on v x ))
+                  (bfr-varname-p v))
+             (not (logicman-pathcond-depends-on v new-logicman)))
+    :hints(("Goal" :in-theory (enable logicman-pathcond-depends-on
+                                      bfr-depends-on
+                                      bfr-varname-p
+                                      bfr-fix
+                                      bfr->aignet-lit)))))
+
+
+                                  
+
+
+    
